fv/lean/Ragu/Instances/Point/Alloc.lean
@@ -7,28 +7,33 @@ open Core.Primes
 @[reducible]
 def CircuitField := F Core.Primes.p
 
-def exported_operations : Operations CircuitField := [
+def Inputs := unit
+
+-- Point allocation instance:
+set_option linter.unusedVariables false in
+def exported_operations (input_var : Var Inputs CircuitField) : Operations CircuitField := [
   Operation.witness 3 (fun _env => default),
-  Operation.assert ((((var 0) * (var 1)) + (0x40000000000000000000000000000000224698fc094cf91b992d30ed00000000 * (var 2)))),
-  Operation.assert (((var 0) + (0x40000000000000000000000000000000224698fc094cf91b992d30ed00000000 * (var 1)))),
+  Operation.assert ((((var 0) * (var 1)) + ((0x40000000000000000000000000000000224698fc094cf91b992d30ed00000000 : Expression CircuitField) * (var 2)))),
+  Operation.assert (((var 0) + ((0x40000000000000000000000000000000224698fc094cf91b992d30ed00000000 : Expression CircuitField) * (var 1)))),
   Operation.witness 3 (fun _env => default),
-  Operation.assert ((((var 3) * (var 4)) + (0x40000000000000000000000000000000224698fc094cf91b992d30ed00000000 * (var 5)))),
-  Operation.assert (((var 3) + (0x40000000000000000000000000000000224698fc094cf91b992d30ed00000000 * (var 0)))),
-  Operation.assert (((var 4) + (0x40000000000000000000000000000000224698fc094cf91b992d30ed00000000 * (var 2)))),
+  Operation.assert ((((var 3) * (var 4)) + ((0x40000000000000000000000000000000224698fc094cf91b992d30ed00000000 : Expression CircuitField) * (var 5)))),
+  Operation.assert (((var 3) + ((0x40000000000000000000000000000000224698fc094cf91b992d30ed00000000 : Expression CircuitField) * (var 0)))),
+  Operation.assert (((var 4) + ((0x40000000000000000000000000000000224698fc094cf91b992d30ed00000000 : Expression CircuitField) * (var 2)))),
   Operation.witness 3 (fun _env => default),
-  Operation.assert ((((var 6) * (var 7)) + (0x40000000000000000000000000000000224698fc094cf91b992d30ed00000000 * (var 8)))),
-  Operation.assert (((var 6) + (0x40000000000000000000000000000000224698fc094cf91b992d30ed00000000 * (var 7)))),
-  Operation.assert ((((var 5) + (0x0000000000000000000000000000000000000000000000000000000000000005 * 1)) + (0x40000000000000000000000000000000224698fc094cf91b992d30ed00000000 * (var 8)))),
+  Operation.assert ((((var 6) * (var 7)) + ((0x40000000000000000000000000000000224698fc094cf91b992d30ed00000000 : Expression CircuitField) * (var 8)))),
+  Operation.assert (((var 6) + ((0x40000000000000000000000000000000224698fc094cf91b992d30ed00000000 : Expression CircuitField) * (var 7)))),
+  Operation.assert ((((var 5) + ((0x0000000000000000000000000000000000000000000000000000000000000005 : Expression CircuitField) * 1)) + ((0x40000000000000000000000000000000224698fc094cf91b992d30ed00000000 : Expression CircuitField) * (var 8)))),
 ]
 
-def exported_output : List (Expression CircuitField) := [(var 0), (var 6)]
+set_option linter.unusedVariables false in
+def exported_output (input_var : Var Inputs CircuitField) : List (Expression CircuitField) := [(var 0), (var 6)]
 
 def EpAffineParams: Circuits.Point.Spec.CurveParams CircuitField := {b := 5}
 
-def circuit := (Circuits.Point.Alloc.circuit EpAffineParams).main (F:=CircuitField) default
+def circuit := (Circuits.Point.Alloc.circuit EpAffineParams).main (F:=CircuitField)
 
-theorem same_circuit :
-    (circuit.operations 0).toFlat = exported_operations.toFlat := by
+theorem same_circuit (input : Var Inputs CircuitField):
+    ((circuit input).operations 0).toFlat = (exported_operations input).toFlat := by
   simp [Operations.toFlat, circuit_norm, FormalCircuit.toSubcircuit,
     circuit,
     Circuits.Point.Alloc.circuit, Circuits.Point.Alloc.elaborated, Circuits.Point.Alloc.main,
@@ -37,9 +42,13 @@ theorem same_circuit :
     Circuits.Element.Mul.circuit, Circuits.Element.Mul.elaborated, Circuits.Element.Mul.main]
   rfl
 
-theorem same_output :
-    (circuit.output 0).x = exported_output[0] ∧
-    (circuit.output 0).y = exported_output[1] := by
+
+lemma exported_output_len (input : Var Inputs CircuitField) : (exported_output input).length = 2 := by
+  simp only [exported_output, List.length_cons, List.length_nil, zero_add, Nat.reduceAdd]
+
+theorem same_output (input : Var Inputs CircuitField) :
+    ((circuit input).output 0).x = (exported_output input)[0]'(by simp [exported_output_len]) ∧
+    ((circuit input).output 0).y = (exported_output input)[1]'(by simp [exported_output_len]) := by
   simp [circuit_norm,
     circuit, exported_output,
     Circuits.Point.Alloc.circuit, Circuits.Point.Alloc.elaborated, Circuits.Point.Alloc.main,
